lt proof almost done

FractionVerification/Basic.lean
@@ -7,6 +7,10 @@ abbrev Fraction := Int128 × UInt128
 
 def Fraction.toRat (r : Fraction) : ℚ := r.1.toInt / r.2.toNat
 
+def Fraction.num (r : Fraction) := r.1
+
+def Fraction.denom (r : Fraction) := r.2
+
 aegis_spec "fraction_verification::abs::abs<core::integer::i128, core::integer::I128PartialOrd, core::integer::I128Neg, core::integer::i128Drop, core::integer::i128Copy, core::integer::I128Zero, core::integer::u128, core::integer::DowncastableIntTryInto<core::integer::i128, core::integer::u128, core::integer::DowncastableI128, core::integer::DowncastableU128, _>>" :=
   fun _ _ a _ ρ =>
   a ≠ BitVec.intMin 128 ∧ ρ = .inl a.abs ∨
@@ -26,8 +30,8 @@ aegis_prove "fraction_verification::abs::abs<core::integer::i128, core::integer:
         bv_decide
       · rcases h₃ with (h₃|h₃)
         · simp [BitVec.slt_iff_toInt_lt, BitVec.sle_iff_toInt_le, BitVec.slt_eq_decide] at *
-          rcases h₂ with ⟨h₂,rfl⟩
-          rcases h₃ with ⟨h₃,rfl⟩
+          rcases h₂ with ⟨-,rfl⟩
+          rcases h₃ with ⟨-,rfl⟩
           simp at h₄
         · simp [BitVec.slt_iff_toInt_lt, BitVec.sle_iff_toInt_le, BitVec.slt_eq_decide] at *
           rcases h₂ with ⟨h₂,rfl⟩
@@ -35,7 +39,7 @@ aegis_prove "fraction_verification::abs::abs<core::integer::i128, core::integer:
           rw [BitVec.toInt_neg_of_ne_intMin h₂] at h₃
           omega
     · rcases h₂ with (h₂|h₂)
-      · rcases h₂ with ⟨h₂,rfl⟩
+      · rcases h₂ with ⟨-,rfl⟩
         simp at h₃
       · rcases h₃ with ⟨rfl,rfl⟩
         rcases h₂ with ⟨rfl,-⟩
@@ -56,20 +60,48 @@ aegis_prove "fraction_verification::abs::AbsImplI128::abs" :=
   unfold_spec "fraction_verification::abs::AbsImplI128::abs"
   aesop
 
+theorem lt_aux1 {x y : BitVec w} (hx : ¬ x.slt 0) (hy : ¬ y.slt 0) : x < y ↔ x.slt y :=
+  ⟨fun h => by bv_decide, fun h => by bv_decide⟩
+
+theorem lt_aux2 {x : BitVec 128} : x.toNat = (0#128 ++ x).toInt := by
+  rw [BitVec.toInt_eq_toNat_of_msb (by bv_decide)]
+  congr 1
+  rw [← BitVec.toNat_setWidth' (n := 256) (by simp), BitVec.toNat_inj,
+    BitVec.setWidth'_eq]
+  bv_decide
+
+theorem lt_aux3 {x : BitVec 128} (hx : (0#128).sle x = «true») : x.toInt = (0#128 ++ x).toInt := by
+  rw [← BitVec.toInt_signExtend_of_le (x := x) (v := 256) (by simp), BitVec.toInt_inj]
+  bv_decide
+
+set_option grind.warning false in
+theorem lt_aux4 {x y : BitVec 256} (h : ¬ x.smulOverflow y) : x.toInt * y.toInt = (x * y).toInt := by
+  rw [@BitVec.toInt_mul]
+  unfold BitVec.smulOverflow at h
+  symm
+  apply Int.bmod_eq_of_le_mul_two
+  <;> grind
+
+theorem lt_aux5 {x : BitVec 128} (h : BitVec.sle 0 x) : x.abs = x := by
+  bv_decide
+
 aegis_spec "fraction_verification::fraction::FractionPartialOrd::lt" :=
   fun _ _ (a b : Fraction) _ ρ =>
+  0 < a.denom → 0 < b.denom →
   ρ = .inl (Bool.toSierraBool (a.toRat < b.toRat)) ∨
     ρ.isRight
 
 set_option maxHeartbeats 1_000_000 in
 --set_option pp.notation false in
+-- set_option profiler true in
 aegis_prove "fraction_verification::fraction::FractionPartialOrd::lt" :=
   fun _ _ (a b : Fraction) _ ρ => by
   unfold_spec "fraction_verification::fraction::FractionPartialOrd::lt"
   rintro ⟨_,_,_,_,_,_,_,_,_,_,h⟩
+  intro ha hb
   rcases h with ⟨_,_,_,_,_,_,_,_,_,_,h⟩
   rcases h with ⟨_,_,_,_,_,_,_,_,_,_,h⟩
-  rcases h with ⟨_,_,_,_,_,_,rfl,(⟨h₁,h₂⟩|h)⟩
+  rcases h with ⟨_,_,_,_,_,_,rfl,(⟨h₁,h₂⟩|⟨h₁,rfl,h₂⟩)⟩
   · rcases h₂ with (⟨h₂,h₃⟩|⟨h₂,rfl,h₃⟩)
     · rcases h₃ with (⟨h₃,rfl,h₅,h₆⟩|⟨h₃,rfl,h₄⟩)
       · rcases h₆ with (⟨rfl,h₇,h₈⟩|⟨rfl,rfl⟩)
@@ -77,19 +109,25 @@ aegis_prove "fraction_verification::fraction::FractionPartialOrd::lt" :=
           · rcases h₁₀ with (⟨rfl,h₁₁,h₁₂⟩|⟨rfl,rfl⟩)
             · rcases h₁₂ with (⟨rfl,h₁₃⟩|⟨rfl,rfl⟩)
               · rcases h₁₃ with (⟨h₁₃,rfl⟩|⟨h₁₃,rfl⟩)
-                · simp at *
+                · simp only [Bool.toSierraBool_iff_eq_false', ne_eq, Nat.ofNat_pos, Sum.inl.injEq,
+                  Sum.isRight_inl, Bool.false_eq_true, and_false, or_false, Nat.reduceAdd,
+                  BitVec.ofNat_eq_ofNat, Bool.not_eq_true, gt_iff_lt] at *
                   rcases h₇ with ⟨h₇,rfl⟩
                   rcases h₁₁ with ⟨h₁₁,rfl⟩
                   congr 2
-                  simp [Fraction.toRat, UInt256.mul_def]
+                  simp only [UInt256.mul_def, Nat.reduceAdd, UInt256.append_ofBitVec,
+                    Fraction.toRat, eq_iff_iff]
                   bv_decide
-                · simp at *
+                · simp only [Bool.toSierraBool_iff_eq_false', ne_eq, Nat.ofNat_pos, Sum.inl.injEq,
+                  Sum.isRight_inl, Bool.false_eq_true, and_false, or_false, Nat.reduceAdd,
+                  BitVec.ofNat_eq_ofNat, Bool.not_eq_true, Bool.toSierraBool_iff_eq_true'] at *
                   rcases h₅ with ⟨h₅,rfl⟩
                   rcases h₇ with ⟨h₇,rfl⟩
                   rcases h₉ with ⟨h₉,rfl⟩
                   rcases h₁₁ with ⟨h₁₁,rfl⟩
                   congr 2
-                  simp [Fraction.toRat, UInt256.mul_def]
+                  simp only [UInt256.mul_def, Nat.reduceAdd, UInt256.append_ofBitVec,
+                    Fraction.toRat, eq_iff_iff]
                   bv_decide
               · simp
             · simp
@@ -101,20 +139,28 @@ aegis_prove "fraction_verification::fraction::FractionPartialOrd::lt" :=
             · rcases h₈ with (⟨rfl,h₈,h₉⟩|⟨rfl,rfl⟩)
               · rcases h₉ with (⟨rfl,h₉⟩|⟨rfl,rfl⟩)
                 · rcases h₉ with (⟨h₉,rfl⟩|⟨h₉,rfl⟩)
-                  · simp at *
+                  · simp only [Bool.toSierraBool_iff_eq_false', Bool.toSierraBool_iff_eq_true',
+                    decide_eq_false_iff_not, ne_eq, Nat.ofNat_pos, Sum.inl.injEq, Sum.isRight_inl,
+                    Bool.false_eq_true, and_false, or_false, Nat.reduceAdd, BitVec.ofNat_eq_ofNat,
+                    Bool.not_eq_true, gt_iff_lt] at *
                     rcases h₆ with ⟨h₆,rfl⟩
                     rcases h₇ with ⟨h₇,rfl⟩
                     rcases h₈ with ⟨h₈,rfl⟩
                     congr 2
-                    simp [Fraction.toRat, UInt256.mul_def]
+                    simp only [UInt256.mul_def, Nat.reduceAdd, UInt256.append_ofBitVec,
+                      Fraction.toRat, eq_iff_iff]
                     bv_decide
-                  · simp at *
+                  · simp only [Bool.toSierraBool_iff_eq_false', Bool.toSierraBool_iff_eq_true',
+                    decide_eq_false_iff_not, ne_eq, Nat.ofNat_pos, Sum.inl.injEq, Sum.isRight_inl,
+                    Bool.false_eq_true, and_false, or_false, Nat.reduceAdd, BitVec.ofNat_eq_ofNat,
+                    Bool.not_eq_true] at *
                     rcases h₅ with ⟨h₅,rfl⟩
                     rcases h₆ with ⟨h₆,rfl⟩
                     rcases h₇ with ⟨h₇,rfl⟩
                     rcases h₈ with ⟨h₈,rfl⟩
                     congr 2
-                    simp [Fraction.toRat, UInt256.mul_def]
+                    simp only [UInt256.mul_def, Nat.reduceAdd, UInt256.append_ofBitVec,
+                      Fraction.toRat, eq_iff_iff]
                     bv_decide
                 · simp
               · simp
@@ -122,10 +168,215 @@ aegis_prove "fraction_verification::fraction::FractionPartialOrd::lt" :=
           · simp
         · simp at *
           bv_decide
-    · rcases h₃ with (h₃|⟨h₃,rfl⟩)
-      · sorry
-      · simp [Fraction.toRat] at *
-        sorry -- lhs neg, rhs pos
-  · sorry --right; aesop
+    · rcases h₃ with (⟨h₃,h₄⟩|⟨h₃,rfl⟩)
+      · rcases h₄ with (⟨h₄,h₅,h₆,h₇⟩|⟨h₄,h₅,h₆⟩)
+        · cases h₅
+          rcases h₇ with (⟨rfl,h₇,h₈⟩|⟨-,rfl⟩)
+          · rcases h₈ with (⟨rfl,h₈,h₉⟩|⟨-,rfl⟩)
+            · rcases h₉ with (⟨rfl,h₉,h₁₀⟩|⟨h₉,rfl⟩)
+              · rcases h₁₀ with (⟨rfl,h₁₀⟩|⟨_,rfl⟩)
+                · rcases h₁₀ with (⟨h₁₀,rfl⟩|⟨h₁₀,rfl⟩)
+                  · simp [Fraction.toRat] at *
+                    bv_decide
+                  · simp [Fraction.toRat, Fraction.denom] at *
+                    rcases h₆ with ⟨h₆,rfl⟩
+                    rcases h₇ with ⟨h₇,rfl⟩
+                    rcases h₈ with ⟨h₈,rfl⟩
+                    rcases h₉ with ⟨h₉,rfl⟩
+                    simp only [UInt256.mul_def, Nat.reduceAdd, UInt256.append_ofBitVec]
+                    congr 2
+                    rw [lt_aux1 (by bv_decide) (by bv_decide), BitVec.slt_iff_toInt_lt]
+                    rw [div_lt_div_iff₀ (by simp [BitVec.lt_def] at ha; erw [Nat.cast_lt]; assumption)
+                        (by simp [BitVec.lt_def] at hb; erw [Nat.cast_lt]; assumption)]
+                    norm_cast
+                    congr
+                    · rw [lt_aux2, lt_aux3 h₂, lt_aux4 (by bv_decide), lt_aux5 h₂]
+                    · rw [lt_aux2, lt_aux3 (by bv_decide), lt_aux4 (by bv_decide), lt_aux5 (by bv_decide)]
+                · right; simp
+              · right; simp
+            · right; simp
+          · right; simp
+        · rcases h₆ with (⟨h₆,h₇,h₈⟩|⟨_,rfl⟩)
+          · cases h₅
+            rcases h₈ with (⟨rfl,h₈,h₉⟩|⟨_,rfl⟩)
+            · rcases h₉ with (⟨rfl,h₉,h₁₀⟩|⟨_,rfl⟩)
+              · rcases h₁₀ with (⟨rfl,h₁₀,h₁₁⟩|⟨_,rfl⟩)
+                · rcases h₁₁ with (⟨rfl,h₁₁⟩|⟨_,rfl⟩)
+                  · rcases h₁₁ with (⟨h₁₁,rfl⟩|⟨h₁₁,rfl⟩)
+                    · simp only [BitVec.ofNat_eq_ofNat, Bool.toSierraBool_iff_eq_false',
+                      Bool.toSierraBool_iff_eq_true', decide_eq_false_iff_not, ne_eq, Nat.ofNat_pos,
+                      Sum.inl.injEq, Sum.isRight_inl, Bool.false_eq_true, and_false, or_false,
+                      Nat.reduceAdd, Bool.not_eq_true, gt_iff_lt, Fraction.toRat] at *
+                      bv_decide
+                    · simp only [BitVec.ofNat_eq_ofNat, Bool.toSierraBool_iff_eq_false',
+                      Bool.toSierraBool_iff_eq_true', decide_eq_false_iff_not, ne_eq, Nat.ofNat_pos,
+                      Sum.inl.injEq, Sum.isRight_inl, Bool.false_eq_true, and_false, or_false,
+                      Nat.reduceAdd, Bool.not_eq_true, Fraction.toRat] at *
+                      bv_decide
+                  · right; simp
+                · right; simp
+              · right; simp
+            · right; simp
+          · cases h₅
+            simp_all
+      · simp [Fraction.toRat, Fraction.denom] at *
+        trans 0
+        · apply div_nonpos_of_nonpos_of_nonneg
+          · norm_cast
+            erw [← BitVec.sle_iff_toInt_le (y := 0#128)]
+            assumption
+          · simp
+        · apply Rat.div_nonneg
+          · norm_cast
+            erw [← BitVec.sle_iff_toInt_le (x := 0#128)]
+            assumption
+          · simp
+  · rcases h₂ with (⟨h₂,h₃⟩|⟨h₂,rfl⟩)
+    · rcases h₃ with (⟨h₃,h₄⟩|h₃)
+      · rcases h₄ with (⟨h₄,h₅,h₆,h₇⟩|⟨h₄,h₅,h₆⟩)
+        · cases h₅
+          rcases h₇ with (⟨rfl,h₇,h₈⟩|⟨_,rfl⟩)
+          · rcases h₈ with (⟨rfl,h₈,h₉⟩|⟨_,rfl⟩)
+            · rcases h₉ with (⟨rfl,h₁₀,h₁₁⟩|⟨_,rfl⟩)
+              · rcases h₁₁ with (⟨rfl,h₁₁⟩|⟨_,rfl⟩)
+                · rcases h₁₁ with (⟨h₁₁,rfl⟩|⟨h₁₁,rfl⟩)
+                  · simp only [BitVec.ofNat_eq_ofNat, Fraction.denom,
+                    Bool.toSierraBool_iff_eq_true', Bool.toSierraBool_iff_eq_false', ne_eq,
+                    Nat.ofNat_pos, Sum.inl.injEq, Sum.isRight_inl, Bool.false_eq_true, and_false,
+                    or_false, Nat.reduceAdd, Bool.not_eq_true, gt_iff_lt, Fraction.toRat] at *
+                    bv_decide
+                  · simp only [BitVec.ofNat_eq_ofNat, Fraction.denom,
+                    Bool.toSierraBool_iff_eq_true', Bool.toSierraBool_iff_eq_false', ne_eq,
+                    Nat.ofNat_pos, Sum.inl.injEq, Sum.isRight_inl, Bool.false_eq_true, and_false,
+                    or_false, Nat.reduceAdd, Bool.not_eq_true, Fraction.toRat] at *
+                    bv_decide
+                · right; simp
+              · right; simp
+            · right; simp
+          · right; simp
+        · cases h₅
+          rcases h₆ with (⟨h₆,h₇,h₈⟩|⟨h₆,rfl⟩)
+          · rcases h₈ with (⟨rfl,h₉,h₁₀⟩|⟨_,rfl⟩)
+            · rcases h₁₀ with (⟨rfl,h₁₀,h₁₁⟩|⟨_,rfl⟩)
+              · rcases h₁₁ with (⟨rfl,h₁₁,h₁₂⟩|⟨_,rfl⟩)
+                · rcases h₁₂ with (⟨rfl,h₁₂⟩|⟨_,rfl⟩)
+                  · rcases h₁₂ with (⟨h₁₂,rfl⟩|⟨h₁₂,rfl⟩)
+                    · simp only [BitVec.ofNat_eq_ofNat, Fraction.denom,
+                      Bool.toSierraBool_iff_eq_true', Bool.toSierraBool_iff_eq_false',
+                      decide_eq_false_iff_not, ne_eq, Nat.ofNat_pos, Sum.inl.injEq, Sum.isRight_inl,
+                      Bool.false_eq_true, and_false, or_false, Nat.reduceAdd, Bool.not_eq_true,
+                      gt_iff_lt, Fraction.toRat] at *
+                      congr 2
+                      rcases h₇ with ⟨h₇,rfl⟩
+                      rcases h₉ with ⟨h₉,rfl⟩
+                      rcases h₁₀ with ⟨h₁₀,rfl⟩
+                      rcases h₁₁ with ⟨h₁₁,rfl⟩
+                      simp [UInt256.mul_def, UInt256.append_ofBitVec]
+                      congr 2
+                      rw [lt_aux1 (by bv_decide) (by bv_decide), BitVec.slt_iff_toInt_lt]
+                      rw [div_lt_div_iff₀ (by simp [BitVec.lt_def] at ha; erw [Nat.cast_lt]; assumption)
+                          (by simp [BitVec.lt_def] at hb; erw [Nat.cast_lt]; assumption)]
+                      norm_cast
+                      sorry
+                    · simp only [BitVec.ofNat_eq_ofNat, Fraction.denom,
+                      Bool.toSierraBool_iff_eq_true', Bool.toSierraBool_iff_eq_false',
+                      decide_eq_false_iff_not, ne_eq, Nat.ofNat_pos, Sum.inl.injEq, Sum.isRight_inl,
+                      Bool.false_eq_true, and_false, or_false, Nat.reduceAdd, Bool.not_eq_true,
+                      Fraction.toRat] at *
+                      bv_decide
+                  · right; simp
+                · right; simp
+              · right; simp
+            · right; simp
+          · simp_all only [BitVec.ofNat_eq_ofNat, Fraction.denom, Bool.toSierraBool_iff_eq_false',
+            Bool.toSierraBool_iff_eq_true', Fraction.toRat, Sum.inl.injEq, decide_eq_true_eq,
+            Sum.isRight_inl, Bool.false_eq_true, or_false, Bool.toSierraBool_true,
+            Bool.toSierraBool_iff_eq_true, Bool.toSierraBool_false, Bool.toSierraBool_iff_eq_false,
+            BitVec.toInt_zero, Int.cast_zero, zero_div]
+            apply div_neg_of_neg_of_pos
+            · norm_cast
+              erw [← BitVec.slt_iff_toInt_lt (y := 0#128)]
+              assumption
+            · norm_cast
+      · rcases h₃ with ⟨h₃,h₄,h₅⟩
+        cases h₄
+        rcases h₅ with (⟨h₅,h₆⟩|⟨h₅,rfl⟩)
+        · rcases h₆ with (⟨h₆,h₇,h₈,h₉⟩|⟨h₆,h₇,h₈⟩)
+            <;> cases h₇
+          · rcases h₉ with (⟨rfl,h₉,h₁₀⟩|⟨_,rfl⟩)
+            · rcases h₁₀ with (⟨rfl,h₁₀,h₁₁⟩|⟨_,rfl⟩)
+              · rcases h₁₁ with (⟨rfl,h₁₁,h₁₂⟩|⟨_,rfl⟩)
+                · rcases h₁₂ with (⟨rfl,h₁₂⟩|⟨_,rfl⟩)
+                  · rcases h₁₂ with (⟨h₁₂,rfl⟩|⟨h₁₂,rfl⟩)
+                    · simp only [BitVec.ofNat_eq_ofNat, Fraction.denom,
+                      Bool.toSierraBool_iff_eq_true', Bool.toSierraBool_iff_eq_false', ne_eq,
+                      Nat.ofNat_pos, Sum.inl.injEq, Sum.isRight_inl, Bool.false_eq_true, and_false,
+                      or_false, Nat.reduceAdd, Bool.not_eq_true, gt_iff_lt, Fraction.toRat] at *
+                      bv_decide
+                    · simp only [BitVec.ofNat_eq_ofNat, Fraction.denom,
+                      Bool.toSierraBool_iff_eq_true', Bool.toSierraBool_iff_eq_false', ne_eq,
+                      Nat.ofNat_pos, Sum.inl.injEq, Sum.isRight_inl, Bool.false_eq_true, and_false,
+                      or_false, Nat.reduceAdd, Bool.not_eq_true, Fraction.toRat] at *
+                      bv_decide
+                  · right; simp
+                · right; simp
+              · right; simp
+            · right; simp
+          · rcases h₈ with (⟨h₈,h₉,h₁₀⟩|⟨h₈,rfl⟩)
+            · rcases h₁₀ with (⟨rfl,h₁₀,h₁₁⟩|⟨_,rfl⟩)
+              · rcases h₁₁ with (⟨rfl,h₁₁,h₁₂⟩|⟨_,rfl⟩)
+                · rcases h₁₂ with (⟨rfl,h₁₂,h₁₃⟩|⟨_,rfl⟩)
+                  · rcases h₁₃ with (⟨rfl,h₁₃⟩|⟨_,rfl⟩)
+                    · rcases h₁₃ with (⟨h₁₃,rfl⟩|⟨h₁₃,rfl⟩)
+                      · simp only [BitVec.ofNat_eq_ofNat, Fraction.denom,
+                        Bool.toSierraBool_iff_eq_true', Bool.toSierraBool_iff_eq_false',
+                        decide_eq_false_iff_not, ne_eq, Nat.ofNat_pos, Sum.inl.injEq,
+                        Sum.isRight_inl, Bool.false_eq_true, and_false, or_false, Nat.reduceAdd,
+                        Bool.not_eq_true, gt_iff_lt, Fraction.toRat] at *
+                        bv_decide
+                      · simp only [BitVec.ofNat_eq_ofNat, Fraction.denom,
+                        Bool.toSierraBool_iff_eq_true', Bool.toSierraBool_iff_eq_false',
+                        decide_eq_false_iff_not, ne_eq, Nat.ofNat_pos, Sum.inl.injEq,
+                        Sum.isRight_inl, Bool.false_eq_true, and_false, or_false, Nat.reduceAdd,
+                        Bool.not_eq_true, Fraction.toRat] at *
+                        bv_decide
+                    · right; simp
+                  · right; simp
+                · right; simp
+              · right; simp
+            · simp only [BitVec.ofNat_eq_ofNat, Fraction.denom, Bool.toSierraBool_iff_eq_true',
+              Bool.toSierraBool_iff_eq_false', decide_eq_true_eq, Fraction.toRat, Sum.inl.injEq,
+              Sum.isRight_inl, Bool.false_eq_true, or_false] at *
+              bv_decide
+        · simp only [BitVec.ofNat_eq_ofNat, Fraction.denom, Bool.toSierraBool_iff_eq_true',
+          Bool.toSierraBool_iff_eq_false', Fraction.toRat, Sum.inl.injEq, decide_eq_false_iff_not,
+          not_lt, Sum.isRight_inl, Bool.false_eq_true, or_false] at *
+          trans 0
+          · apply div_nonpos_of_nonpos_of_nonneg <;> norm_cast
+            · erw [← BitVec.sle_iff_toInt_le (y := 0#128)]
+              assumption
+            · erw [← BitVec.le_def (x := 0#128)]
+              bv_decide
+          · apply le_of_eq
+            symm
+            rw [div_eq_zero_iff]
+            left
+            norm_cast
+            erw [BitVec.toInt_inj (y := 0#128)]
+            bv_decide
+    · simp only [BitVec.ofNat_eq_ofNat, Fraction.denom, Bool.toSierraBool_iff_eq_true',
+      Fraction.toRat, Sum.inl.injEq, decide_eq_true_eq, Sum.isRight_inl, Bool.false_eq_true,
+      or_false] at *
+      apply lt_of_le_of_lt
+      · apply div_nonpos_of_nonpos_of_nonneg
+        · norm_cast
+          erw [← BitVec.sle_iff_toInt_le (y := 0#128)]
+          assumption
+        · simp
+      · apply div_pos
+        · norm_cast
+          erw [← BitVec.slt_iff_toInt_lt (x := 0#128)]
+          assumption
+        · norm_cast
 
 aegis_complete
